Inserted an explicit meta-reset in the classical case of soundness of reset. Cleaned up a bit.

coq/nbe_shift_1/nbe_cbn.ml
@@ -157,7 +157,7 @@ module type Kripke_structure =
   
   val coq_X_mon2 : coq_K -> bool -> formula -> coq_X -> bool -> coq_X
   
-  val coq_X_reset : coq_K -> coq_X -> coq_X
+  val coq_X_reset : coq_K -> bool -> coq_X -> coq_X
  end
 
 module Kripke_structure_monad = 
@@ -360,7 +360,8 @@ module Coq_sforces_cbn =
          Obj.magic (fun w'' w'w'' k ->
            Coq_ks.coq_X_mon2 w'' False Bot
              (Obj.magic h Bot w'' w'w'' (fun w2 w''w2 hA ->
-               Coq_ks.coq_X_reset w2 (k w2 w''w2 (sforces_mon3 w2 hA)))) True)
+               Coq_ks.coq_X_reset w2 False (k w2 w''w2 (sforces_mon3 w2 hA))))
+             True)
        | False -> h)
   
   (** val sforces_mon2 : formula -> Coq_ks.coq_K -> sforces -> sforces **)
@@ -458,11 +459,12 @@ module Soundness =
         (match annot' with
          | True ->
            Obj.magic
-             (Coq_cbn_validity.run w True
-               (soundness gamma True Bot p0 w True h'))
+             (Coq_ks.coq_X_reset w True
+               (Coq_cbn_validity.run w True
+                 (soundness gamma True Bot p0 w True h')))
          | False ->
            Obj.magic
-             (Coq_ks.coq_X_reset w
+             (Coq_ks.coq_X_reset w False
                (Coq_cbn_validity.run w True
                  (soundness gamma True Bot p0 w True
                    (Coq_generic_properties.coq_Kont_sforces_cxt_mon2 gamma w
@@ -525,10 +527,10 @@ module Completeness =
       | Bot -> Obj.magic (proof_ne_mon2 Bot w annot (Obj.magic h) annot')
       | x -> Obj.magic (proof_nf_mon2 x w annot (Obj.magic h) annot')
     
-    (** val coq_X_reset : context -> proof_ne -> proof_ne **)
+    (** val coq_X_reset : context -> bool -> proof_ne -> proof_ne **)
     
-    let coq_X_reset w h =
-      Ne_Reset (w, False, h)
+    let coq_X_reset w annot h =
+      Ne_Reset (w, annot, h)
    end
   
   module Coq_ks_monad = Kripke_structure_monad(U)
